Commiting changes for new meta-extract mods: one book changed by me, the rest courtesy of Sol Swords.
(Sol)  clause-processors/meta-extract-user.lisp
(Sol)  centaur/misc/context-rw.lisp
(Sol)  centaur/misc/interp-function-lookup.lisp
(Sol)  centaur/gl/def-gl-clause-proc.lisp
(Matt) system/meta-extract.lisp

books/system/meta-extract.lisp
@@ -6,4 +6,4 @@
 
 (verify-termination meta-extract-contextual-fact)
 
-(verify-termination meta-extract-global-fact)
+(verify-termination meta-extract-global-fact+)
